introduce nat_TM locale (with sublocale)
define conversion functions `f, g` with `SOME` (similar for their inverses), prove properties later
create sublocale similar to the rejecting TM, but introduce as named sublocale ("natM") to avoid "Duplicate constant declaration". this allows using shorthand versions of locale definitions for both the original TM `M` (`halts w`) and the new `natM` (`natM.halts w`)

papers/116_stefan_rass/TM.thy
@@ -615,38 +615,45 @@ end \<comment> \<open>\<^locale>\<open>Rej_TM\<close>\<close>
 subsection\<open>(nat, nat) TM\<close>
 text \<open>Every well-formed TM is equivalent to some (nat, nat) TM\<close>
 
-context TM begin
+locale nat_TM = TM +
+  fixes f :: "'a \<Rightarrow> nat" and f_inv
+    and g :: "'b \<Rightarrow> nat" and g_inv
+  defines "f \<equiv> SOME f. inj_on f (states M)"  and "f_inv \<equiv> the_inv_into (states M) f"
+    and   "g \<equiv> SOME g. inj_on g (symbols M)" and "g_inv \<equiv> the_inv_into (symbols M) g"
+begin
 
-(* TODO: split into multiple lemmas *)
-lemma natify:
-  obtains natM :: "(nat, nat) TM" and f :: "'a \<Rightarrow> nat" and g :: "'b \<Rightarrow> nat"
-  where "inj_on f (states M)" and "inj_on g (symbols M)"
-  and "TM natM"
-  and "\<And>w. halts w \<Longrightarrow> TM.halts natM (map g w)"
-  and "\<And>w. accepts w \<Longrightarrow> TM.accepts natM (map g w)"
-  and "\<And>w. rejects w \<Longrightarrow> TM.rejects natM (map g w)"
-proof
-  obtain f :: "'a \<Rightarrow> nat" where "inj_on f (states M)"
-    using countable_finite[OF state_axioms(1)] unfolding countable_def ..
-  define f_inv :: "nat \<Rightarrow> 'a" where "f_inv \<equiv> the_inv_into (states M) f"
+lemma f_inj: "inj_on f (states M)" unfolding f_def
+  using countable_finite[OF state_axioms(1)] unfolding countable_def ..
+lemma "q \<in> states M \<Longrightarrow> f_inv (f q) = q" unfolding f_inv_def
+  using f_inj by (rule the_inv_into_f_f)
 
-  obtain g :: "'b \<Rightarrow> nat" where "inj_on g (symbols M)"
-    using countable_finite[OF symbol_axioms(1)] unfolding countable_def ..
-  define g_inv :: "nat \<Rightarrow> 'b" where "g_inv \<equiv> the_inv_into (symbols M) g"
+lemma g_inj: "inj_on g (symbols M)" unfolding g_def
+  using countable_finite[OF symbol_axioms(1)] unfolding countable_def ..
+lemma "\<sigma> \<in> symbols M \<Longrightarrow> g_inv (g \<sigma>) = \<sigma>" unfolding g_inv_def
+  using g_inj by (rule the_inv_into_f_f)
 
-  define natM :: "(nat, nat) TM" where "natM \<equiv> \<lparr>
-      tape_count = tape_count M,
-      states = f ` states M,
-      start_state = f (start_state M),
-      final_states = f ` (final_states M),
-      accepting_states = f ` (accepting_states M),
-      symbols = g ` (symbols M),
-      next_state = \<lambda>q w. f (next_state M (f_inv q) (map g_inv w)),
-      next_action = \<lambda>q w. map (action_app g) (next_action M (f_inv q) (map g_inv w))
+definition natM :: "(nat, nat) TM" ("M\<^sub>\<nat>")
+  where "natM \<equiv> \<lparr>
+    tape_count = tape_count M,
+    states = f ` states M,
+    start_state = f (start_state M),
+    final_states = f ` (final_states M),
+    accepting_states = f ` (accepting_states M),
+    symbols = g ` (symbols M),
+    next_state = \<lambda>q w. f (next_state M (f_inv q) (map g_inv w)),
+    next_action = \<lambda>q w. map (action_app g) (next_action M (f_inv q) (map g_inv w))
   \<rparr>"
 
-qed
+(* using the same name ("natM") for both sublocale and definition works,
+ * since the sublocale is only used as namespace *)
+sublocale natM: TM natM
+  sorry
 
-end
+lemma "\<And>w. halts w \<Longrightarrow> natM.halts (map g w)"
+  and "\<And>w. accepts w \<Longrightarrow> natM.accepts (map g w)"
+  and "\<And>w. rejects w \<Longrightarrow> natM.rejects (map g w)"
+  sorry
+
+end \<comment> \<open>\<^locale>\<open>nat_TM\<close>\<close>
 
 end
